1) Fixed rmap to be parial 2) simplified simulation relations, s.t. they consider both value_id and value_const cases, which reduces 1/3 size of the proofs
Checkpoint before another change.

Here is the problem. The SoftBound instrumentation of malloc is like
this:
%p = malloc i8, i32 (ptrtoint (i32* (inttoptr (i32 42 to i32*)) %to i32))
%b = bitcast i8* %p to i8*
%e = gep i8* %p, i32 (ptrtoint (i32* (inttoptr (i32 42 to i32*)) %to i32))

[NOTE: The ptrtoint and inttoptr things are optimized away by llvm-as
-disable-opt. From the log of llvm-as, I cannot find which pass it runs
to do such constant-fold. Maybe by default such folding should happen.
So we cannot create a case to show the problem.]

In term of the current memory model, if 42 is not a valid address for
any allocated blocks, inttoptr returns null, and the final reresult
before malloc is 0. Suppose the malloc turns 42 to be an allocated
address, the constant returns 42 after the malloc. This is inconsistent
with LLVM.

To fix it, we are intruducing a new value, Vint2ptr : int -> val. Given
an inttoptr i, if the i is within a good memory block b with ofs, it
returns Vptr b ofs, otherwise it returns Vint2ptr i. In such an way, we
turned int2ptr to be total w/o losing any information.



git-svn-id: https://webdav.seas.upenn.edu/svn/sol/vol@2886 eef5ea85-cc2e-0410-bd84-0fae1f012da8

src/SoftBound/sb_def.v
@@ -54,25 +54,16 @@ match c with
 | _ => None
 end.
 
-Definition get_reg_metadata TD M gl (rm:rmetadata) (v:value) : metadata :=
+Definition get_reg_metadata TD M gl (rm:rmetadata) (v:value) : option metadata :=
   match v with
-  | value_id pid => 
-      match lookupAL _ rm pid with
-      | Some md => md
-      | None => mkMD null null
-      end
+  | value_id pid => lookupAL _ rm pid
   | value_const c => 
       match get_const_metadata c with
       | Some (bc, ec) => 
-          match 
-            (do gvb <- const2GV TD M gl bc;
-             do gve <- const2GV TD M gl ec;
-             ret (mkMD gvb gve))
-          with
-          | Some (mkMD gvb gve) => mkMD gvb gve
-          | None => mkMD null null
-          end
-      | None => mkMD null null
+          do gvb <- const2GV TD M gl bc;
+          do gve <- const2GV TD M gl ec;
+          ret (mkMD gvb gve)
+      | None => Some (mkMD null null)
       end
   end.
 
@@ -223,7 +214,7 @@ Inductive dbCmd : TargetData -> GVMap ->
     trace_nil rerror
 
 | dbLoad_nptr : forall TD rm lc gl id t vp align Mem MM als gvp md gv,
-  get_reg_metadata TD Mem gl rm vp = md ->
+  get_reg_metadata TD Mem gl rm vp = Some md ->
   getOperandValue TD Mem vp lc gl = Some gvp ->
   assert_mptr TD t gvp md ->
   mload TD Mem gvp t align = Some gv ->
@@ -232,7 +223,7 @@ Inductive dbCmd : TargetData -> GVMap ->
     rm als Mem MM trace_nil rok
 
 | dbLoad_ptr : forall TD rm lc gl id t vp align Mem MM als gvp md gv md' lc' rm',
-  get_reg_metadata TD Mem gl rm vp = md ->
+  get_reg_metadata TD Mem gl rm vp = Some md ->
   getOperandValue TD Mem vp lc gl = Some gvp ->
   assert_mptr TD t gvp md ->
   mload TD Mem gvp t align = Some gv ->
@@ -264,14 +255,14 @@ Inductive dbCmd : TargetData -> GVMap ->
     trace_nil rerror
 
 | dbLoad_abort : forall TD rm lc gl id t vp align Mem MM als gvp md,
-  get_reg_metadata TD Mem gl rm vp = md ->
+  get_reg_metadata TD Mem gl rm vp = Some md ->
   getOperandValue TD Mem vp lc gl = Some gvp ->
   ~ assert_mptr TD t gvp md ->
   dbCmd TD gl lc rm als Mem MM (insn_load id t vp align) lc rm als Mem MM
     trace_nil rabort
 
 | dbStore_nptr : forall TD rm lc gl sid t v vp align Mem MM als gv gvp md Mem',
-  get_reg_metadata TD Mem gl rm vp = md ->
+  get_reg_metadata TD Mem gl rm vp = Some md ->
   getOperandValue TD Mem v lc gl = Some gv ->
   getOperandValue TD Mem vp lc gl = Some gvp ->
   assert_mptr TD t gvp md ->
@@ -282,13 +273,13 @@ Inductive dbCmd : TargetData -> GVMap ->
 
 | dbStore_ptr : forall TD rm lc gl sid t v vp align Mem MM als gv gvp md Mem' 
                        md' MM',
-  get_reg_metadata TD Mem gl rm vp = md ->
+  get_reg_metadata TD Mem gl rm vp = Some md ->
   getOperandValue TD Mem v lc gl = Some gv ->
   getOperandValue TD Mem vp lc gl = Some gvp ->
   assert_mptr TD t gvp md ->
   mstore TD Mem gvp t gv align = Some Mem' ->
   isPointerTyp t ->
-  get_reg_metadata TD Mem gl rm v = md' ->
+  get_reg_metadata TD Mem gl rm v = Some md' ->
   set_mem_metadata TD MM gvp md' = MM' -> 
   dbCmd TD gl lc rm als Mem MM (insn_store sid t v vp align) lc rm als Mem' MM'
     trace_nil rok
@@ -320,7 +311,7 @@ Inductive dbCmd : TargetData -> GVMap ->
     trace_nil rerror
 
 | dbStore_abort : forall TD rm lc gl sid t v vp align Mem MM als gv gvp md,
-  get_reg_metadata TD Mem gl rm vp = md ->
+  get_reg_metadata TD Mem gl rm vp = Some md ->
   getOperandValue TD Mem v lc gl = Some gv ->
   getOperandValue TD Mem vp lc gl = Some gvp ->
   ~ assert_mptr TD t gvp md ->
@@ -330,7 +321,7 @@ Inductive dbCmd : TargetData -> GVMap ->
 
 | dbGEP : forall TD rm lc gl id inbounds t vp idxs vidxs gvp' Mem MM als gvp md 
                  lc' rm',
-  get_reg_metadata TD Mem gl rm vp = md ->
+  get_reg_metadata TD Mem gl rm vp = Some md ->
   getOperandValue TD Mem vp lc gl = Some gvp ->
   values2GVs TD Mem idxs lc gl = Some vidxs ->
   GEP TD t gvp vidxs inbounds = Some gvp' ->
@@ -374,7 +365,7 @@ Inductive dbCmd : TargetData -> GVMap ->
 | dbBitcast_ptr : forall TD rm lc gl id t1 v1 t2 gv2 Mem MM als lc' md rm',
   CAST TD Mem lc gl castop_bitcast t1 v1 t2 = Some gv2 ->
   isPointerTyp t1 ->
-  get_reg_metadata TD Mem gl rm v1 = md ->
+  get_reg_metadata TD Mem gl rm v1 = Some md ->
   prop_reg_metadata lc rm id gv2 md = (lc', rm') ->
   dbCmd TD gl lc rm als Mem MM (insn_cast id castop_bitcast t1 v1 t2) lc' rm' 
     als Mem MM trace_nil rok
@@ -426,8 +417,8 @@ Inductive dbCmd : TargetData -> GVMap ->
                  rm',
   SELECT TD Mem v0 v1 v2 lc gl = Some gv ->
   isPointerTyp t ->
-  get_reg_metadata TD Mem gl rm v1 = md1 ->
-  get_reg_metadata TD Mem gl rm v2 = md2 ->
+  get_reg_metadata TD Mem gl rm v1 = Some md1 ->
+  get_reg_metadata TD Mem gl rm v2 = Some md2 ->
   getOperandValue TD Mem v0 lc gl = Some cond ->
   (if isGVZero TD cond then 
     prop_reg_metadata lc rm id gv md2
@@ -511,8 +502,8 @@ Definition callUpdateLocals (TD:TargetData) (M:mem) (noret:bool) (rid:id)
         | Some Result => 
           match (getOperandValue TD M Result lc' gl) with 
           | Some gr => 
-              let md' := get_reg_metadata TD M gl rm' Result in
-               Some (updateAddAL _ lc rid gr, updateAddAL _ rm rid md')
+              do md' <- get_reg_metadata TD M gl rm' Result;
+              ret (updateAddAL _ lc rid gr, updateAddAL _ rm rid md')
           | None => None
           end
         end
@@ -524,7 +515,7 @@ Fixpoint initRmetadata_aux TD Mem gl (la:args) (lp:params) (rm accum:rmetadata)
 match (la, lp) with
 | ((t,id)::la', (_,v)::lp') =>
     if isPointerTypB t then
-      let md := get_reg_metadata TD Mem gl rm v in 
+      do md <- get_reg_metadata TD Mem gl rm v;
       initRmetadata_aux TD Mem gl la' lp' rm (updateAddAL _ accum id md)
     else initRmetadata_aux TD Mem gl la' lp' rm accum
 | (nil, nil) => Some accum
