src/SoftBound/sbop_seop.v
@@ -94,6 +94,8 @@ Proof.
   destruct oResult; try solve [inversion H; subst; auto].
   destruct (getOperandValue TD Mem'' v lc' gl); 
     try solve [inversion H; subst; auto].
+  destruct (SoftBound.get_reg_metadata TD Mem'' gl rm' v); 
+    try solve [inversion H; subst; auto].
 Qed.
 
 Definition sbop_dbCall__seop_dbCall_prop S TD Ps fs gl lc rm Mem0 MM0 call0 lc'
